Add schedule-based optimiser and further real-identity rewrites

icing/source_to_sourceScript.sml
@@ -6,7 +6,7 @@
   icing_rewriterScript implementing pattern matching and pattern instantiation.
 *)
 open semanticPrimitivesTheory evaluateTheory terminationTheory
-     icing_rewriterTheory icing_optimisationsTheory;
+     icing_rewriterTheory icing_optimisationsTheory fpOptTheory fpValTreeTheory;
 
 open preamble;
 
@@ -103,6 +103,580 @@ Termination
       \\ first_x_assum (qspec_then `mod` assume_tac) \\ fs[])
 End
 
+(* Datatype for opt_path into a tree value. Here is the leaf node meaning that the
+  rewrite should be applied *)
+val _ = Hol_datatype ‘
+         opt_path =   Left of opt_path | Right of opt_path | Center of opt_path | ListIndex of (num # opt_path) | Here’;
+
+Type fp_plan = “: (opt_path # (fp_pat # fp_pat) list) list”
+
+Definition MAP_plan_to_path_def:
+  MAP_plan_to_path (to_path: opt_path -> opt_path) (plan: fp_plan) = MAP (λ (path, rws). (to_path path, rws)) plan
+End
+
+Definition left_def:
+  left path = Left path
+End
+
+Definition right_def:
+  right path = Right path
+End
+
+Definition center_def:
+  center path = Center path
+End
+
+Definition listIndex_def:
+  listIndex i path = ListIndex (i, path)
+End
+
+Definition canonicalize_sub_def:
+(* Canonicalize sub to add and mul times -1.0 *)
+  canonicalize_sub e =
+    case e of
+    | (App (FP_bop FP_Sub) [e1; e2]) =>
+        (App (FP_bop FP_Add) [e1; rewriteFPexp [fp_neg_times_minus_one] e2],
+         [(Here, [fp_sub_add]); (ListIndex (1, Here),  [fp_neg_times_minus_one])])
+    | _ => (e, [])
+End
+
+Definition canonicalize_app_def:
+  canonicalize_app e =
+    case e of
+    (* Canonicalize to right associative *)
+    | (App (FP_bop op) [App (FP_bop op2) [e1_1; e1_2]; e2]) =>
+        (if (op = op2 ∧ op ≠ FP_Sub ∧ op ≠ FP_Div) then
+           let (local_rewritten, local_plan) =
+               (App (FP_bop op) [e1_1; App (FP_bop op2) [e1_2; e2]], [(Here, [fp_assoc_gen op])]) in
+             case local_rewritten of
+             | App (FP_bop op) [e1'; e2'] =>
+                 (let (child_rewritten, child_plan) = canonicalize_app e2' in
+                    (App (FP_bop op) [e1'; child_rewritten],
+                     local_plan ++ (MAP_plan_to_path (listIndex 1) child_plan)))
+             | _ => (local_rewritten, local_plan)
+         else (canonicalize_sub e))
+    (* Canonicalize constants to the rhs *)
+    | (App (FP_bop op) [App FpFromWord [l]; e2]) =>
+        (if (op ≠ FP_Sub ∧ op ≠ FP_Div) then
+           (rewriteFPexp [fp_comm_gen op] e, [(Here, [fp_comm_gen op])])
+         else
+           (e, []))
+    | (App (FP_bop FP_Sub) [e1; e2]) =>
+        canonicalize_sub e
+    | _ => (e, [])
+Termination
+  WF_REL_TAC ‘measure (λe. exp_size e)’ \\ fs[]
+  \\ rpt strip_tac
+  \\ fs[astTheory.exp_size_def]
+  \\ fs[astTheory.op_size_def, fpValTreeTheory.fp_bop_size_def]
+End
+
+Definition canonicalize_def:
+  canonicalize (cfg: config) (FpOptimise sc e) = (
+  let (e_can, plan: fp_plan) = canonicalize (cfg with canOpt := if sc = Opt then T else F) e in
+    (FpOptimise sc e_can, MAP_plan_to_path center plan)
+  ) ∧
+  canonicalize cfg (App op exps) = (
+    let individuals = MAP (canonicalize cfg) exps in
+      let exps_can = MAP FST individuals;
+          plan: fp_plan = FLAT ( MAPi (λ i (_, plani). MAP_plan_to_path (listIndex i) plani) individuals ) in
+        if (cfg.canOpt) then
+          let (new_e, can_plan) = canonicalize_app (App op exps_can) in
+            (new_e, plan ++ can_plan)
+        else (App op exps_can, plan)
+    ) ∧
+  canonicalize cfg (Let so e1 e2) = (
+    let (e1_can, plan_left) = canonicalize cfg e1;
+        (e2_can, plan_right) = canonicalize cfg e2 in
+        (Let so e1_can e2_can, (MAP_plan_to_path left plan_left) ++ (MAP_plan_to_path right plan_right))
+    ) ∧
+  canonicalize cfg (Con mod exps) = (
+    let (individuals: (exp # (opt_path # (fp_pat # fp_pat) list) list) list) = MAP (canonicalize cfg) exps in
+      let exps_can = MAP FST individuals;
+          plan = FLAT ( MAPi (λ i (_, plani). MAP_plan_to_path (listIndex i) plani) individuals ) in
+        (Con mod exps_can, plan)
+    ) ∧
+  canonicalize cfg (Log lop e2 e3) = (
+    let (e2_can, plan_left) = canonicalize cfg e2;
+        (e3_can, plan_right) = canonicalize cfg e3 in
+      (Log lop e2_can e3_can, (MAP_plan_to_path left plan_left) ++ (MAP_plan_to_path right plan_right))
+    ) ∧
+  canonicalize cfg (If e1 e2 e3) = (
+    let (e1_can, plan_left) = canonicalize cfg e1;
+        (e2_can, plan_center) = canonicalize cfg e2;
+        (e3_can, plan_right) = canonicalize cfg e3 in
+      (If e1_can e2_can e3_can,
+       (MAP_plan_to_path left plan_left)
+       ++
+       (MAP_plan_to_path center plan_center)
+       ++
+       (MAP_plan_to_path right plan_right))
+    ) ∧
+  canonicalize cfg (Lannot e l) = (
+    let (e_can, plan_center) = canonicalize cfg e in
+      (Lannot e_can l, MAP_plan_to_path center plan_center)
+    ) ∧
+  canonicalize cfg (Tannot e t) = (
+    let (e_can, plan_center) = canonicalize cfg e in
+      (Tannot e_can t, MAP_plan_to_path center plan_center)
+    ) ∧
+  canonicalize cfg (Letrec ses e) = (
+    let (e_can, plan_center) = canonicalize cfg e in
+      (Letrec ses e_can, MAP_plan_to_path center plan_center)
+    ) ∧
+  canonicalize cfg (Mat e pes) = (
+    let (e_can, plan_left) = canonicalize cfg e;
+        individuals = MAP (λ (p, e'). (p, canonicalize cfg e')) pes in
+      let pes_can = MAP (λ(p, (e', _)). (p, e')) individuals;
+          pes_plan = FLAT (MAPi (λ i (_, (_, plani)). MAP_plan_to_path (listIndex i) plani) individuals);
+          e_plan = MAP_plan_to_path left plan_left in
+        (Mat e_can pes_can, e_plan ++ pes_plan)
+    ) ∧
+  (* We do not apply any canonicalization plan to the rest *)
+  canonicalize cfg e = (e, [])
+Termination
+  WF_REL_TAC ‘measure (λ (cfg, e). exp_size e)’ \\ fs[]
+  \\ strip_tac
+  >- (
+  Induct_on ‘pes’ \\ fs[]
+  \\ rpt strip_tac \\ rveq
+  \\ first_x_assum (qspecl_then [‘e’, ‘cfg’, ‘e_can’, ‘plan_left’, ‘p’, ‘e'’] strip_assume_tac)
+  \\ pop_assum imp_res_tac \\ fs[astTheory.exp_size_def]
+  )
+  >- (
+  strip_tac
+  \\ Induct_on ‘exps’ \\ fs[]
+  \\ rpt strip_tac \\ fs[astTheory.exp_size_def]
+  >- (
+    first_x_assum (qspecl_then [‘op’, ‘a’] strip_assume_tac)
+    \\ pop_assum imp_res_tac \\ fs[]
+    )
+  \\ qpat_x_assum ‘∀ mod a. _ ⇒ exp_size a < _’ (qspecl_then [‘mod’, ‘a’] strip_assume_tac)
+  \\ pop_assum imp_res_tac \\ fs[]
+  )
+End
+
+
+Theorem test__canonicalize = EVAL (
+  Parse.Term ‘
+   canonicalize no_fp_opt_conf (
+     (FpOptimise Opt
+      (App (FP_bop FP_Add) [
+         App (FP_bop FP_Add) [
+             App (FP_bop FP_Add) [
+                 App (FP_bop FP_Add) [
+                     Var (Short "c");
+                     Var (Short "d")
+                   ];
+                 Var (Short "b")
+               ];
+             App (FP_bop FP_Mul) [
+                 Var (Short "x");
+                 Var (Short "y")
+               ]
+           ];
+         Var (Short "a")
+        ])
+     )
+     )
+  ’);
+
+
+Definition post_order_dfs_for_plan_def:
+  post_order_dfs_for_plan (f: config -> exp -> (exp # fp_plan) option) (cfg: config) (FpOptimise sc e) = (
+  let (e_can, plan: fp_plan) = post_order_dfs_for_plan f (cfg with canOpt := if sc = Opt then T else F) e in
+    ((FpOptimise sc e_can), MAP (λ (path, rws). (Center path, rws)) plan)
+  ) ∧
+  post_order_dfs_for_plan f cfg (App op exps) = (
+    let individuals = MAP (post_order_dfs_for_plan f cfg) exps in
+      let exps_can = MAP FST individuals;
+          plan: fp_plan = FLAT ( MAPi (λ i (_, plani). MAP_plan_to_path (listIndex i) plani) individuals ) in
+        if (cfg.canOpt) then
+          case f cfg (App op exps_can) of
+          | (SOME (new_e, can_plan)) => (new_e, plan ++ can_plan)
+          | NONE => (App op exps_can, plan)
+         else (App op exps_can, plan)
+    ) ∧
+  post_order_dfs_for_plan f cfg (Let so e1 e2) = (
+    let (e1_can, plan_left) = post_order_dfs_for_plan f cfg e1;
+        (e2_can, plan_right) = post_order_dfs_for_plan f cfg e2 in
+        (Let so e1_can e2_can, (MAP_plan_to_path left plan_left) ++ (MAP_plan_to_path right plan_right))
+    ) ∧
+  post_order_dfs_for_plan f cfg (Con mod exps) = (
+    let (individuals: (exp # (opt_path # (fp_pat # fp_pat) list) list) list) =
+        MAP (post_order_dfs_for_plan f cfg) exps in
+      let exps_can = MAP FST individuals;
+          plan = FLAT ( MAPi (λ i (_, plani). MAP_plan_to_path (listIndex i) plani) individuals ) in
+        (Con mod exps_can, plan)
+    ) ∧
+  post_order_dfs_for_plan f cfg (Log lop e2 e3) = (
+    let (e2_can, plan_left) = post_order_dfs_for_plan f cfg e2;
+        (e3_can, plan_right) = post_order_dfs_for_plan f cfg e3 in
+      (Log lop e2_can e3_can, (MAP_plan_to_path left plan_left) ++ (MAP_plan_to_path right plan_right))
+    ) ∧
+  post_order_dfs_for_plan f cfg (If e1 e2 e3) = (
+    let (e1_can, plan_left) = post_order_dfs_for_plan f cfg e1;
+        (e2_can, plan_center) = post_order_dfs_for_plan f cfg e2;
+        (e3_can, plan_right) = post_order_dfs_for_plan f cfg e3 in
+      (If e1_can e2_can e3_can,
+       (MAP_plan_to_path left plan_left)
+       ++
+       (MAP_plan_to_path center plan_center)
+       ++
+       (MAP_plan_to_path right plan_right))
+    ) ∧
+  post_order_dfs_for_plan f cfg (Lannot e l) = (
+    let (e_can, plan_center) = post_order_dfs_for_plan f cfg e in
+      (Lannot e_can l, MAP_plan_to_path center plan_center)
+    ) ∧
+  post_order_dfs_for_plan f cfg (Tannot e t) = (
+    let (e_can, plan_center) = post_order_dfs_for_plan f cfg e in
+      (Tannot e_can t, MAP_plan_to_path center plan_center)
+    ) ∧
+  post_order_dfs_for_plan f cfg (Letrec ses e) = (
+    let (e_can, plan_center) = post_order_dfs_for_plan f cfg e in
+      (Letrec ses e_can, MAP_plan_to_path center plan_center)
+    ) ∧
+  post_order_dfs_for_plan f cfg (Mat e pes) = (
+    let (e_can, plan_left) = post_order_dfs_for_plan f cfg e;
+        individuals = MAP (λ (p, e'). (p,  post_order_dfs_for_plan f cfg e')) pes in
+      let pes_can = MAP (λ(p, (e', _)). (p, e')) individuals;
+          pes_plan = FLAT (MAPi (λ i (_, (_, plani)). MAP_plan_to_path (listIndex i) plani) individuals);
+          e_plan = MAP_plan_to_path left plan_left in
+        (Mat e_can pes_can, e_plan ++ pes_plan)
+    ) ∧
+  (* We do not apply any canonicalization plan to the rest *)
+  post_order_dfs_for_plan f cfg e = (e, [])
+Termination
+  WF_REL_TAC ‘measure (λ (f, cfg, e). exp_size e)’ \\ fs[]
+  \\ strip_tac
+  >- (
+  Induct_on ‘pes’ \\ fs[]
+  \\ rpt strip_tac \\ rveq
+  \\ first_x_assum (qspecl_then [‘e’, ‘cfg’, ‘f’, ‘e_can’, ‘plan_left’, ‘p’, ‘e'’] strip_assume_tac)
+  \\ pop_assum imp_res_tac \\ fs[astTheory.exp_size_def]
+  )
+  >- (
+  strip_tac
+  \\ Induct_on ‘exps’ \\ fs[]
+  \\ rpt strip_tac \\ fs[astTheory.exp_size_def]
+  >- (
+    first_x_assum (qspecl_then [‘op’, ‘a’] strip_assume_tac)
+    \\ pop_assum imp_res_tac \\ fs[]
+    )
+  \\ qpat_x_assum ‘∀ mod a. _ ⇒ exp_size a < _’ (qspecl_then [‘mod’, ‘a’] strip_assume_tac)
+  \\ pop_assum imp_res_tac \\ fs[]
+  )
+End
+
+
+Definition perform_rewrites_def:
+  (* Make sure not to optimise away the FpOptimise or Let *)
+  perform_rewrites (cfg: config) Here rewrites (FpOptimise sc e) = FpOptimise sc e ∧
+  perform_rewrites (cfg: config) Here rewrites (Let so e1 e2) = Let so e1 e2 ∧
+
+  (* Otherwise, we may optimise everything if we are at the end of the path *)
+  perform_rewrites cfg Here rewrites e = (if (cfg.canOpt) then (rewriteFPexp rewrites e) else e) ∧
+
+  (* If we are not at the end of the path, further navigate through the AST *)
+  perform_rewrites cfg (Left _) rewrites (Lit l) = Lit l ∧
+  perform_rewrites cfg (Left _) rewrites (Var x) = Var x ∧
+  perform_rewrites cfg (Center path) rewrites (Raise e) =
+    Raise (perform_rewrites cfg path rewrites e) ∧
+  (* We cannot support "Handle" expressions because we must be able to reorder exceptions *)
+  perform_rewrites cfg path rewrites (Handle e pes) = Handle e pes ∧
+  perform_rewrites cfg (ListIndex (i, path)) rewrites (Con mod exps) =
+    Con mod (MAPi (λ n e. (if (n = i) then (perform_rewrites cfg path rewrites e) else e)) exps) ∧
+  (* TODO: Why is this not optimized? *)
+  perform_rewrites cfg (Left _) rewrites (Fun s e) = Fun s e ∧
+  perform_rewrites cfg (ListIndex (i, path)) rewrites (App op exps) =
+    App op (MAPi (λ n e. (if (n = i) then (perform_rewrites cfg path rewrites e) else e)) exps) ∧
+  perform_rewrites cfg (Left path) rewrites (Log lop e2 e3) =
+    Log lop (perform_rewrites cfg path rewrites e2) e3 ∧
+  perform_rewrites cfg (Right path) rewrites (Log lop e2 e3) =
+    Log lop e2 (perform_rewrites cfg path rewrites e3) ∧
+  perform_rewrites cfg (Left path) rewrites (If e1 e2 e3) =
+    If (perform_rewrites cfg path rewrites e1) e2 e3 ∧
+  perform_rewrites cfg (Center path) rewrites (If e1 e2 e3) =
+    If e1 (perform_rewrites cfg path rewrites e2) e3 ∧
+  perform_rewrites cfg (Right path) rewrites (If e1 e2 e3) =
+    If e1 e2 (perform_rewrites cfg path rewrites e3) ∧
+  perform_rewrites cfg (Left path) rewrites (Mat e pes) = Mat (perform_rewrites cfg path rewrites e) pes ∧
+  perform_rewrites cfg (ListIndex (i, path)) rewrites (Mat e pes) =
+    Mat e (MAPi (λ n (p, e'). (if (n = i) then (p, (perform_rewrites cfg path rewrites e')) else (p, e'))) pes) ∧
+  perform_rewrites cfg (Left path) rewrites (Let so e1 e2) =
+    Let so (perform_rewrites cfg path rewrites e1) e2 ∧
+  perform_rewrites cfg (Right path) rewrites (Let so e1 e2) =
+    Let so e1 (perform_rewrites cfg path rewrites e2) ∧
+  perform_rewrites cfg (Center path) rewrites (Letrec ses e) =
+    Letrec ses (perform_rewrites cfg path rewrites e) ∧
+  perform_rewrites cfg (Center path) rewrites (Tannot e t) =
+    Tannot (perform_rewrites cfg path rewrites e) t ∧
+  perform_rewrites cfg (Center path) rewrites (Lannot e l) =
+    Lannot (perform_rewrites cfg path rewrites e) l ∧
+  perform_rewrites cfg (Center path) rewrites (FpOptimise sc e) =
+    FpOptimise sc (perform_rewrites (cfg with canOpt := if sc = Opt then T else F) path rewrites e) ∧
+  perform_rewrites cfg _ _ e = e
+End
+
+Definition optimise_with_plan_def:
+  optimise_with_plan cfg [] e = e ∧
+  optimise_with_plan cfg ((path, rewrites)::rest) e = optimise_with_plan cfg rest (perform_rewrites cfg path rewrites e)
+End
+
+
+Definition optimise_linear_interpolation_def:
+  optimise_linear_interpolation cfg e =
+  post_order_dfs_for_plan (λ cfg e.
+                             (* Does it match  *)
+                             case (matchesFPexp (Binop FP_Add
+                                                 (Binop FP_Mul
+                                                  (Var 0)
+                                                  (Binop FP_Sub
+                                                   (Word (4607182418800017408w: word64))
+                                                   (Var 1)))
+                                                 (Binop FP_Mul
+                                                  (Var 2)
+                                                  (Var 1))) e []) of
+                             | SOME _ =>
+                                 let plan = [
+                                     (ListIndex (0, Here), [fp_comm_gen FP_Mul;
+                                                            fp_undistribute_gen FP_Mul FP_Sub;
+                                                            fp_comm_gen FP_Mul;
+                                                            fp_sub_add ]);
+                                     (Here, [fp_assoc_gen FP_Add]);
+                                     (ListIndex (1, Here), [fp_neg_push_mul_r]);
+                                     (ListIndex (1, ListIndex (0, Here)), [fp_comm_gen FP_Mul]);
+                                     (ListIndex (1, Here), [fp_distribute_gen FP_Mul FP_Add]);
+                                     (ListIndex (1, (ListIndex (0, Here))), [fp_comm_gen FP_Add; fp_add_sub]);
+                                     (ListIndex (0, Here), [fp_comm_gen FP_Mul; fp_times_one]);
+                                     (ListIndex (1, Here), [fp_comm_gen FP_Mul])
+                                   ] in
+                                   SOME (optimise_with_plan cfg plan e, plan)
+                             | NONE => NONE) cfg e
+End
+
+(*
+Get all top-level multiplicants:
+e.g. for ((x + 0) * (y * (a * 7))), this returns [x+0; y; a; 7].
+This function requires the input to be canonicalized to right-associative.
+*)
+Definition top_level_multiplicants_def:
+  top_level_multiplicants e = case e of
+                              | App (FP_bop FP_Mul) [e1; App (FP_bop FP_Mul) [e1'; e2']] =>
+                                  let vs = (top_level_multiplicants e2') in (e1::e1'::vs)
+                              | App (FP_bop FP_Mul) [e1; e2] => [e1; e2]
+                              | _ => [e]
+End
+
+Theorem test__top_level_multiplicants = EVAL (
+  Parse.Term ‘
+  top_level_multiplicants (App (FP_bop FP_Mul) [
+                               App (FP_bop FP_Add) [Var (Short "x"); Lit (Word64 0w)];
+                               (App (FP_bop FP_Mul) [
+                                   Var (Short "y");
+                                   App (FP_bop FP_Mul) [
+                                       (Var (Short "a"));
+                                       (Lit (Word64 7w))
+                                     ]
+                                 ]
+                               )
+                             ])
+  ’)
+
+Definition remove_first_def:
+  remove_first [] a = [] ∧
+  remove_first (x::rest) a = if (x = a) then rest else x::(remove_first rest a)
+End
+
+Definition intersect_lists_def:
+  intersect_lists _ [] = [] ∧
+  intersect_lists [] _ = [] ∧
+  intersect_lists (a::rest) right =
+  case MEM a right of T => a::(intersect_lists rest (remove_first right a))
+                   | F => intersect_lists rest right
+End
+
+Definition move_multiplicants_to_right_def:
+  move_multiplicants_to_right cfg [] e = (e, []) ∧
+  move_multiplicants_to_right cfg [m] e =
+  (case e of
+   | (App (FP_bop FP_Mul) [e1; e2]) =>
+       if (m = e1) then
+         let plan =  [(Here, [fp_comm_gen FP_Mul])] in
+           let commuted = optimise_with_plan cfg plan e in
+             (commuted, plan)
+       else (
+         if (m = e2) then
+           let local_plan = [(Here, [fp_assoc2_gen FP_Mul])] in
+             (optimise_with_plan cfg local_plan e, local_plan)
+         else
+           let local_plan = [(Here, [fp_assoc2_gen FP_Mul])];
+               (updated_e2, downstream_plan) = move_multiplicants_to_right cfg [m] e2 in
+             let updated_e = App (FP_bop FP_Mul) [e1; updated_e2] in
+               (optimise_with_plan cfg local_plan updated_e,
+                (MAP_plan_to_path (listIndex 1) downstream_plan) ++ local_plan)
+         )
+   | _ => (e, [])) ∧
+  move_multiplicants_to_right cfg (m1::m2::rest) e =
+  let (updated_e, plan) = move_multiplicants_to_right cfg [m1] e in
+    case updated_e of
+    | (App (FP_bop FP_Mul) [e1; e2]) =>
+        (let (updated_e1, other_plan) = move_multiplicants_to_right cfg (m2::rest) e1 in
+           let left_plan = MAP_plan_to_path (listIndex 0) other_plan;
+               local_plan = [(Here, [fp_assoc_gen FP_Mul])] in
+             let final_e = optimise_with_plan cfg local_plan (App (FP_bop FP_Mul) [updated_e1; e2]) in
+               (final_e, plan ++ left_plan ++ local_plan))
+    | _ => (updated_e, plan)
+End
+
+
+Theorem test__move_multiplicants_to_right = EVAL (
+  Parse.Term ‘
+   move_multiplicants_to_right (no_fp_opt_conf with canOpt := T) [(Var (Short "d")); (Var (Short "b"))] (
+     (App (FP_bop FP_Mul) [
+         Var (Short "a");
+         App (FP_bop FP_Mul) [
+             Var (Short "b");
+             App (FP_bop FP_Mul) [
+                 Var (Short "c");
+                 App (FP_bop FP_Mul) [
+                     Var (Short "d");
+                     Var (Short "e")
+                   ]
+               ]
+           ]
+       ])
+     )
+  ’);
+
+Definition canonicalize_for_distributivity_def:
+  canonicalize_for_distributivity cfg e =
+  post_order_dfs_for_plan (λ cfg e.
+                             case e of
+                             | App (FP_bop op) [e1; e2] =>
+                                 if (op = FP_Add ∨ op = FP_Sub)
+                                 then
+                                   let multiplicants1 = top_level_multiplicants e1;
+                                       multiplicants2 = top_level_multiplicants e2 in
+                                     let common_multiplicants = intersect_lists multiplicants1 multiplicants2
+                                     in
+                                       let (e1_to_right, e1_plan) =
+                                           move_multiplicants_to_right cfg common_multiplicants e1;
+                                           (e2_to_right, e2_plan) =
+                                           move_multiplicants_to_right cfg common_multiplicants e2
+                                       in
+                                         let updated_e = App (FP_bop op) [e1_to_right; e2_to_right];
+                                             plan = (MAP_plan_to_path (listIndex 0) e1_plan)
+                                                    ++ (MAP_plan_to_path (listIndex 1) e2_plan) in
+                                           SOME (updated_e, plan)
+                                 else
+                                   NONE
+                             | _ => NONE) cfg e
+End
+
+
+Theorem test__canonicalize_for_distributivity = EVAL (
+  Parse.Term ‘
+   canonicalize_for_distributivity no_fp_opt_conf (
+     (FpOptimise Opt
+      (App (FP_bop FP_Add) [
+          (App (FP_bop FP_Mul) [
+              Var (Short "a");
+              App (FP_bop FP_Mul) [
+                  Var (Short "b");
+                  App (FP_bop FP_Mul) [
+                      Var (Short "c");
+                      App (FP_bop FP_Mul) [
+                          Var (Short "d");
+                          Var (Short "e")
+                        ]
+                    ]
+                ]
+            ]);
+          (App (FP_bop FP_Mul) [
+              Var (Short "q");
+              App (FP_bop FP_Mul) [
+                  Var (Short "b");
+                  App (FP_bop FP_Mul) [
+                      App (FP_bop FP_Sub) [
+                          App (FP_bop FP_Mul) [
+                              Var (Short "d");
+                              Var (Short "c")
+                            ];
+                          App (FP_bop FP_Mul) [
+                              Var (Short "b");
+                              Var (Short "d")
+                            ]
+                        ];
+                      App (FP_bop FP_Mul) [
+                          Var (Short "d");
+                          Var (Short "d")
+                        ]
+                    ]
+                ]
+            ])
+        ])
+     )
+     )
+  ’);
+
+Definition apply_distributivity_def:
+  apply_distributivity cfg e =
+  post_order_dfs_for_plan (λ cfg e.
+                             let (can_e, can_plan) = canonicalize_for_distributivity cfg e in
+                               case can_e of
+                               | App (FP_bop op) [
+                                   App (FP_bop op') [e1_1;e1_2];
+                                   App (FP_bop op'') [e2_1;e2_2]] =>
+                                   if ((op = FP_Add ∨ op = FP_Sub) ∧ (op' = FP_Mul ∨ op' = FP_Div) ∧ op'' = op')
+                                   then
+                                     (let plan = [(Here, [fp_distribute_gen op' op])] in
+                                        let optimized = optimise_with_plan cfg plan can_e in
+                                          SOME (optimized, can_plan ++ plan)
+                                     )
+                                   else NONE
+                               | _ => NONE
+                          ) cfg e
+End
+
+Definition compose_plan_generation_def:
+  compose_plan_generation [] e = (λ cfg. (e, [])) ∧
+  compose_plan_generation ((generator: config -> exp -> (exp # fp_plan))::rest) e =
+  (λ cfg.
+     let (updated_e, plan) = (generator cfg e) in
+        let (final_e, rest_plan) = ((compose_plan_generation rest updated_e) cfg) in
+        (final_e, plan ++ rest_plan)
+  )
+End
+
+(**
+We generate the plan for a single expression. This will get more complicated than only canonicalization.
+**)
+Definition generate_plan_exp_def:
+  generate_plan_exp (cfg: config) (e: exp) = SND (compose_plan_generation [
+                                                     canonicalize;
+                                                     apply_distributivity;
+                                                     canonicalize;
+                                                     optimise_linear_interpolation;
+                                                     canonicalize
+                                                   ] e cfg)
+End
+
+Definition generate_plan_exps_def:
+  generate_plan_exps cfg [] = [] ∧
+  generate_plan_exps cfg [Fun s e] = generate_plan_exps cfg [e] ∧
+  generate_plan_exps cfg (e1::(e2::es)) = (generate_plan_exps cfg [e1]) ++ (generate_plan_exps cfg (e2::es)) ∧
+  generate_plan_exps cfg [e] = generate_plan_exp cfg e
+End
+
+Definition generate_plan_decs_def:
+  generate_plan_decs cfg [] = [] ∧
+  generate_plan_decs cfg [Dlet loc p e] = [generate_plan_exps cfg [e]] ∧
+  generate_plan_decs cfg (d1::(d2::ds)) = (generate_plan_decs cfg [d1]) ++ (generate_plan_decs cfg (d2::ds)) ∧
+  generate_plan_decs cfg [d] = []
+End
+
 (**
   Step 2: Lifting of optimise to expression lists
   stos_pass walks over a list of expressions and calls optimise on
@@ -115,6 +689,15 @@ Definition stos_pass_def:
   stos_pass cfg [Fun s e] =
     [Fun s (HD (stos_pass cfg [e]))] ∧
   stos_pass cfg [e] = [optimise cfg e]
+End
+
+Definition stos_pass_with_plans_def:
+  stos_pass_with_plans cfg plans [] = [] ∧
+  stos_pass_with_plans cfg (plan1::rest) (e1::e2::es) =
+    (stos_pass_with_plans cfg [plan1] [e1]) ++ (stos_pass_with_plans cfg rest (e2::es)) ∧
+  stos_pass_with_plans cfg plans [Fun s e] = [Fun s (HD (stos_pass_with_plans cfg plans [e]))] ∧
+  stos_pass_with_plans cfg [plan] [e] = [optimise_with_plan cfg plan e] ∧
+  stos_pass_with_plans _ _ exps = exps
 End
 
 (* Step 3: Disallow further optimisations *)
@@ -184,6 +767,15 @@ Definition stos_pass_decs_def:
   stos_pass_decs cfg [d] = [d]
 End
 
+Definition stos_pass_with_plans_decs_def:
+  stos_pass_with_plans_decs cfg plans [] = [] ∧
+  stos_pass_with_plans_decs cfg (plans1::rest) (d1::d2::ds) =
+    (stos_pass_with_plans_decs cfg [plans1] [d1] ++ stos_pass_with_plans_decs cfg rest (d2::ds)) ∧
+  stos_pass_with_plans_decs cfg [plans1] [Dlet loc p e] =
+    [Dlet loc p (HD (stos_pass_with_plans cfg [plans1] [e]))] ∧
+  stos_pass_with_plans_decs cfg plans [d] = [d]
+End
+
 Definition no_opt_decs_def:
   no_opt_decs cfg [] = [] ∧
   no_opt_decs cfg (e1::e2::es) =
@@ -194,6 +786,193 @@ Definition no_opt_decs_def:
     [Dletrec ls (MAP (λ (fname, param, e). (fname, param, HD (no_optimise_pass cfg [e]))) exps)] ∧
   no_opt_decs cfg [d] = [d]
 End
+
+
+val test_code =
+(** REPLACE AST BELOW THIS LINE **)
+“[Dlet unknown_loc (Pvar "rigidBody")
+(Fun "x1" (Fun "x2" (Fun "x3" (FpOptimise Opt
+(App (FP_bop FP_Sub)
+  [
+    (App (FP_bop FP_Add)
+    [
+      (App (FP_bop FP_Sub)
+      [
+        (App (FP_bop FP_Add)
+        [
+          (App (FP_bop FP_Mul)
+          [
+            (App (FP_bop FP_Mul)
+            [
+              (App (FP_bop FP_Mul)
+              [
+                (App FpFromWord [Lit (Word64 (4611686018427387904w:word64))]);
+                Var (Short  "x1")
+              ]);
+              Var (Short  "x2")
+            ]);
+            Var (Short  "x3")
+          ]);
+          (App (FP_bop FP_Mul)
+          [
+            (App (FP_bop FP_Mul)
+            [
+              (App FpFromWord [Lit (Word64 (4613937818241073152w:word64))]);
+              Var (Short  "x3")
+            ]);
+            Var (Short  "x3")
+          ])
+        ]);
+        (App (FP_bop FP_Mul)
+        [
+          (App (FP_bop FP_Mul)
+          [
+            (App (FP_bop FP_Mul)
+            [
+              Var (Short  "x2");
+              Var (Short  "x1")
+            ]);
+            Var (Short  "x2")
+          ]);
+          Var (Short  "x3")
+        ])
+      ]);
+      (App (FP_bop FP_Mul)
+      [
+        (App (FP_bop FP_Mul)
+        [
+          (App FpFromWord [Lit (Word64 (4613937818241073152w:word64))]);
+          Var (Short  "x3")
+        ]);
+        Var (Short  "x3")
+      ])
+    ]);
+    Var (Short  "x2")
+  ])))))]”
+
+
+Definition theAST_def:
+  theAST =
+  ^test_code
+End
+
+(** Optimizations to be applied by Icing **)
+Definition theOpts_def:
+  theOpts = extend_conf no_fp_opt_conf
+  [
+    fp_comm_gen FP_Add;
+    fp_fma_intro
+  ]
+End
+
+Theorem theAST_plan = EVAL (Parse.Term ‘generate_plan_decs theOpts theAST’);
+
+(** The code below stores in theorem theAST_opt the optimized version of the AST
+    from above and in errorbounds_AST the inferred FloVer roundoff error bounds
+ **)
+Theorem theAST_opt =
+  EVAL
+    (Parse.Term ‘
+      (no_opt_decs theOpts (stos_pass_with_plans_decs theOpts (generate_plan_decs theOpts theAST) theAST))’);
+
+
+Theorem only_opt_body = EVAL (
+  Parse.Term ‘
+   compose_plan_generation [
+       canonicalize;
+       apply_distributivity;
+       canonicalize;
+       optimise_linear_interpolation;
+       canonicalize
+     ] (
+     (FpOptimise Opt
+      (App (FP_bop FP_Sub)
+       [
+         (App (FP_bop FP_Add)
+          [
+            (App (FP_bop FP_Sub)
+             [
+               (App (FP_bop FP_Add)
+                [
+                  (App (FP_bop FP_Mul)
+                   [
+                     (App (FP_bop FP_Mul)
+                      [
+                        (App (FP_bop FP_Mul)
+                         [
+                           (App FpFromWord [Lit (Word64 (4611686018427387904w:word64))]);
+                           Var (Short  "x1")
+                         ]);
+                        Var (Short  "x2")
+                      ]);
+                     Var (Short  "x3")
+                   ]);
+                  (App (FP_bop FP_Mul)
+                   [
+                     (App (FP_bop FP_Mul)
+                      [
+                        (App FpFromWord [Lit (Word64 (4613937818241073152w:word64))]);
+                        Var (Short  "x3")
+                      ]);
+                     Var (Short  "x3")
+                   ])
+                ]);
+               (App (FP_bop FP_Mul)
+                [
+                  (App (FP_bop FP_Mul)
+                   [
+                     (App (FP_bop FP_Mul)
+                      [
+                        Var (Short  "x2");
+                        Var (Short  "x1")
+                      ]);
+                     Var (Short  "x2")
+                   ]);
+                  Var (Short  "x3")
+                ])
+             ]);
+            (App (FP_bop FP_Mul)
+             [
+               (App (FP_bop FP_Mul)
+                [
+                  (App FpFromWord [Lit (Word64 (4613937818241073152w:word64))]);
+                  Var (Short  "x3")
+                ]);
+               Var (Short  "x3")
+             ])
+          ]);
+         Var (Short  "x2")
+       ]))
+     ) theOpts’
+  );
+
+Definition linear_interpolation_def:
+     linear_interpolation = FpOptimise Opt
+     (App (FP_bop FP_Add)
+      [
+        (App (FP_bop FP_Mul)
+         [
+           Var (Short "y");
+           (App (FP_bop FP_Sub)
+            [
+              (App FpFromWord [Lit (Word64 (4607182418800017408w: word64))]);
+              Var (Short "z")
+            ])
+         ]);
+        (App (FP_bop FP_Mul)
+         [
+           Var (Short "x");
+           Var (Short "z")
+         ])
+      ])
+End
+
+Theorem opt_linint_test_only_opt = EVAL (
+  Parse.Term ‘
+     (optimise_linear_interpolation theOpts linear_interpolation)
+  ’);
+
+
 
 (**
   Translation from floats to reals, needed for correctness proofs, thus we
